code/hash-new/Hacl.Hash.fst
@@ -72,10 +72,10 @@ let update_multi_sha2_512: update_multi_st SHA2_512 =
   Tactics.(synth_by_tactic
     (specialize (mk_update_multi SHA2_512 Hacl.SHA2.update_512) [`%mk_update_multi]))
 
-let update_multi_sha1: update_multi_t SHA1 =
+let update_multi_sha1: update_multi_st SHA1 =
   Tactics.(synth_by_tactic
     (specialize (mk_update_multi SHA1 Hacl.SHA1.update) [`%mk_update_multi]))
 
-let update_multi_md5: update_multi_t MD5 =
+let update_multi_md5: update_multi_st MD5 =
   Tactics.(synth_by_tactic
     (specialize (mk_update_multi MD5 Hacl.MD5.update) [`%mk_update_multi]))
