code/hash-new/Hacl.Hash.fsti
@@ -17,18 +17,6 @@ inline_for_extraction
 let blocks_t (a: hash_alg) =
   b:B.buffer U8.t { B.length b % size_block a = 0 }
 
-// Generic stateful type for update, for any hash_alg.
-inline_for_extraction
-let update_st (a:hash_alg) =
-  s:state a ->
-  block:B.buffer U8.t { B.length block = size_block a } ->
-  ST.Stack unit
-    (requires (fun h ->
-      B.live h s /\ B.live h block /\ B.disjoint s block))
-    (ensures (fun h0 _ h1 ->
-      B.(modifies (loc_buffer s) h0 h1) /\
-      B.as_seq h1 s == Spec.Hash.update a (B.as_seq h0 s) (B.as_seq h0 block)))
-
 // Note: we cannot take more than 4GB of data because we are currently
 // constrained by the size of buffers...
 inline_for_extraction
@@ -51,3 +39,5 @@ val update_multi_sha2_224: update_multi_st SHA2_224
 val update_multi_sha2_256: update_multi_st SHA2_256
 val update_multi_sha2_384: update_multi_st SHA2_384
 val update_multi_sha2_512: update_multi_st SHA2_512
+val update_multi_sha1: update_multi_st SHA1
+val update_multi_md5: update_multi_st MD5
